wip

src/Std/Data/DTreeMap/Slice.lean
@@ -144,6 +144,14 @@ public theorem step_rxcIterator_eq_match' {α β} {cmp : α → α → Ordering}
   rw [step_rxcIterator_eq_match]
   sorry
 
+public theorem val_step_rxcIterator_eq_match' {α β} {cmp : α → α → Ordering} [TransCmp cmp] {it : Iter (α := RxcIterator α β cmp) _} :
+    it.step.val = (match it.internalState.next.filter (fun e => (cmp e.fst it.internalState.bound).isLE) with
+      | some next =>
+        .yield ⟨it.internalState.treeMap, it.internalState.treeMap.getEntryGT? next.fst, it.internalState.bound, (by apply getEntryGE?_getEntryGT?_eq_some)⟩ next
+      | none =>
+        .done ) := by
+  sorry
+
 -- public theorem RxcIterator.induct {α β} {cmp : α → α → Ordering} [TransCmp cmp]
 --     (motive : Iter (α := RxcIterator α β cmp) _ → Sort x)
 --     (step : (it : Iter (α := RxcIterator α β cmp) _) →
@@ -151,6 +159,189 @@ public theorem step_rxcIterator_eq_match' {α β} {cmp : α → α → Ordering}
 --     {it : Iter (α := RxcIterator α β cmp) _}
 
 end Rxc
+
+public structure RocSliceData (α : Type u) (β : α → Type v)
+    (cmp : α → α → Ordering := by exact compare) where
+  treeMap : DTreeMap α β cmp
+  range : Roc α
+
+public abbrev RocSlice α β cmp := Slice (RocSliceData α β cmp)
+
+public instance : Roc.Sliceable (DTreeMap α β cmp) α (RocSlice α β cmp) where
+  mkSlice carrier range := ⟨carrier, range⟩
+
+@[always_inline]
+public def RocSlice.Internal.iterM (s : RocSlice α β cmp) : IterM (α := RxcIterator α β cmp) Id ((a : α) × β a) :=
+  ⟨⟨s.1.treeMap, s.1.treeMap.getEntryGT? s.1.range.lower, s.1.range.upper,
+      by apply getEntryGE?_getEntryGT?_eq_some⟩⟩
+
+public instance {s : RocSlice α β cmp} : ToIterator s Id ((a : α) × β a) where
+  State := RxcIterator α β cmp
+  /-
+  There is a good reason to extract the iterator into a separate function `RccSlice.Internal.iterM`:
+  The `Iterator` instance on `ToIterator.State` needs to unfold `ToIterator.State`, which requires
+  unfolding this `ToIterator` instance. In consequence, the definition of `iterMInternal` is also
+  unfolded. Because it is complex and highly dependent, this is not desirable.
+  See `Std.Iterators.instIteratorState`.
+  -/
+  iterMInternal := RocSlice.Internal.iterM s
+
+#eval (.ofList [⟨0, 0⟩, ⟨1, 1⟩, ⟨100, 3⟩, ⟨101, 4⟩] : DTreeMap Nat (fun _ => Nat) compare)[1<...=102].toList
+
+public theorem step_iter_rocSlice_eq_match {α β} {cmp : α → α → Ordering} [TransCmp cmp] {t : DTreeMap α β cmp} {a b : α} :
+    t[a<...=b].iter.step = (match h : t.getEntryGT? a with
+      | some next =>
+        if h' : (cmp next.fst b).isLE then
+          .yield ⟨t, t.getEntryGT? next.fst, b, (by apply getEntryGE?_getEntryGT?_eq_some)⟩ next
+            (by simp [Iter.IsPlausibleStep, IterM.IsPlausibleStep, Iterator.IsPlausibleStep, Slice.iter_eq_toIteratorIter, ToIterator.iter_eq, RocSlice.Internal.iterM, Roc.Sliceable.mkSlice, Iter.toIterM, IterM.toIter, h', h])
+        else
+          .done (by simpa [Iter.IsPlausibleStep, IterM.IsPlausibleStep, Iterator.IsPlausibleStep, Slice.iter_eq_toIteratorIter, ToIterator.iter_eq, RocSlice.Internal.iterM, Roc.Sliceable.mkSlice, h] using h')
+      | none =>
+        .done (by simp [Iter.IsPlausibleStep, IterM.IsPlausibleStep, Iterator.IsPlausibleStep, Slice.iter_eq_toIteratorIter, ToIterator.iter_eq, RocSlice.Internal.iterM, Roc.Sliceable.mkSlice, h])) := by
+  simp only [Iter.step, PlausibleIterStep.yield, PlausibleIterStep.done]
+  rw [step_rxcIterator_eq_match]
+  simp only [PlausibleIterStep.yield, PlausibleIterStep.done, Id.run_pure]
+  simp only [RocSlice.Internal.iterM, Iter.toIterM, Slice.iter_eq_toIteratorIter, ToIterator.iter_eq, IterM.toIter]
+  simp [Roc.Sliceable.mkSlice]
+  split <;> rename_i heq
+  · simp only [Slice.iter_eq_toIteratorIter, ToIterator.iter_eq, IterM.toIter, RocSlice.Internal.iterM] at heq
+    split <;> split <;> simp_all [IterM.toIter]
+  · simp only [Slice.iter_eq_toIteratorIter, ToIterator.iter_eq, IterM.toIter, RocSlice.Internal.iterM] at heq
+    split <;> simp_all
+
+public theorem val_step_iter_rocSlice_eq_match {α β} {cmp : α → α → Ordering} [TransCmp cmp] {t : DTreeMap α β cmp} {a b : α} :
+    t[a<...=b].iter.step.val = (match t.getEntryGT? a with
+      | some next =>
+        if (cmp next.fst b).isLE then
+          .yield ⟨t, t.getEntryGT? next.fst, b, (by apply getEntryGE?_getEntryGT?_eq_some)⟩ next
+        else
+          .done
+      | none =>
+        .done) := by
+  rw [step_iter_rocSlice_eq_match]
+  split <;> split <;> simp_all
+
+public theorem val_step_iter_rocSlice_eq_match' {α β} {cmp : α → α → Ordering} [TransCmp cmp] {t : DTreeMap α β cmp} {a b : α} :
+    t[a<...=b].iter.step.val = (match (t.getEntryGT? a).filter (fun e => (cmp e.fst b).isLE) with
+      | some next =>
+        .yield ⟨t, t.getEntryGT? next.fst, b, (by apply getEntryGE?_getEntryGT?_eq_some)⟩ next
+      | none =>
+        .done) := by
+  rw [val_step_iter_rocSlice_eq_match]
+  split
+  · split <;> simp_all [Option.filter_some]
+  · simp_all
+
+public theorem filter_toList_eq_match_lt_and_isLE {α β} {cmp : α → α → Ordering} [TransCmp cmp] {t : DTreeMap α β cmp} {a b : α} :
+    t.toList.filter (fun e => cmp a e.fst = .lt ∧ (cmp e.fst b).isLE) = (match (t.getEntryGT? a).filter (fun e => (cmp e.fst b).isLE) with
+      | some next =>
+        next :: t.toList.filter (fun e => cmp next.fst e.fst = .lt ∧ (cmp e.fst b).isLE)
+      | none =>
+        []) := by
+  induction hs : t.size
+  · rw [← beq_iff_eq, ← DTreeMap.isEmpty_eq_size_eq_zero] at hs
+    have : t.toList = [] := by simpa [← DTreeMap.isEmpty_toList] using hs
+    simp [getEntryGT?_of_isEmpty hs, this]
+  · sorry
+
+public theorem toList_rocSlice_eq_filter_toList {α β} {cmp : α → α → Ordering} [TransCmp cmp]
+    {t : DTreeMap α β cmp} {a b : α} :
+    t[a<...=b].toList = t.toList.filter (fun e => cmp a e.fst = .lt ∧ (cmp e.fst b).isLE) := by
+  rw [filter_toList_eq_match_lt_and_isLE, Slice.toList_eq_toList_iter, Iter.toList_eq_match_step,
+    val_step_iter_rocSlice_eq_match']
+  cases Option.filter (fun e => (cmp e.fst b).isLE) (t.getEntryGT? a)
+  · simp
+  · rename_i next
+    suffices h : t[next.fst<...=b].toList = t.toList.filter (fun e => cmp next.fst e.fst = .lt ∧ (cmp e.fst b).isLE) by
+      simpa [Slice.toList_eq_toList_iter, Slice.iter_eq_toIteratorIter, ToIterator.iter_eq,
+        RocSlice.Internal.iterM, Roc.Sliceable.mkSlice] using h
+    apply toList_rocSlice_eq_filter_toList
+termination_by (t.toList.filter (fun e => cmp a e.fst = .lt ∧ (cmp e.fst b).isLE)).length
+decreasing_by
+  rename_i next hnext
+  simp
+  simp only [getEntryGT?_eq_some_iff, Option.filter_eq_some_iff] at hnext
+  apply List.length_filter_strict_mono (a := next)
+  · simp
+    intro e hne heb
+    exact ⟨TransCmp.lt_trans hnext.1.2.1 hne, heb⟩
+  · exact hnext.1.1
+  · simp [ReflCmp.compare_self]
+  · simp
+    exact ⟨hnext.1.2.1, hnext.2⟩
+
+theorem toList_rocSlice_eq_toList_rocSlice {α β} {cmp : α → α → Ordering} [TransCmp cmp] {t t': DTreeMap α β cmp} {a b a' b' : α}
+    (h : ∀ c, (c ∈ t.toList ∧ cmp a c.fst = .lt ∧ (cmp c.fst b).isLE) ↔ (c ∈ t'.toList ∧ cmp a' c.fst = .lt ∧ (cmp c.fst b').isLE)) :
+    t[a<...=b].toList = t'[a'<...=b'].toList := by
+    -- simp only [Slice.toList_eq_toList_iter, Slice.iter_eq_toIteratorIter, ToIterator.iter_eq,
+    --   RccSlice.Internal.iterM, Rcc.Sliceable.mkSlice, IterM.toIter]
+    simp only [Slice.toList_eq_toList_iter]
+    generalize hi : Slice.iter (Roc.Sliceable.mkSlice t a<...=b) = it
+    change Iter (α := RxcIterator α β cmp) _ at it
+    induction it using Iter.inductSteps generalizing a b a' b' with | step it ihy ihs
+    rw [← hi]
+    simp only [Slice.iter_eq_toIteratorIter, ToIterator.iter_eq, RocSlice.Internal.iterM, Roc.Sliceable.mkSlice, IterM.toIter]
+    rw [Iter.toList_eq_match_step, Iter.toList_eq_match_step]
+    rw [val_step_rxcIterator_eq_match', val_step_rxcIterator_eq_match']
+    simp only
+    have : (t.getEntryGT? a).filter (fun e => (cmp e.fst b).isLE) =
+        (t'.getEntryGT? a').filter (fun e => (cmp e.fst b').isLE) := by
+      ext e
+      simp [getEntryGT?_eq_some_iff]
+      specialize h
+      constructor
+      · intro h'
+        have he := (h e).mp ⟨h'.1.1, h'.1.2.1, h'.2⟩
+        refine ⟨⟨he.1, he.2.1, ?_⟩, he.2.2⟩
+        intro k hk hk'
+        by_cases hkb : (cmp k b').isLE
+        · simp only [← map_fst_toList_eq_keys, List.mem_map] at hk
+          obtain ⟨f, hfm, rfl⟩ := hk
+          have hf := (h f).mpr ⟨hfm, hk', hkb⟩
+          apply h'.1.2.2
+          · simpa only [← map_fst_toList_eq_keys] using List.mem_map_of_mem hf.1
+          · exact hf.2.1
+        · refine TransCmp.isLE_trans he.2.2 ?_
+          apply Ordering.isLE_of_eq_lt
+          simpa [OrientedCmp.gt_iff_lt] using hkb
+      · intro h'
+        have he := (h e).mpr ⟨h'.1.1, h'.1.2.1, h'.2⟩
+        refine ⟨⟨he.1, he.2.1, ?_⟩, he.2.2⟩
+        intro k hk hk'
+        by_cases hkb : (cmp k b).isLE
+        · simp only [← map_fst_toList_eq_keys, List.mem_map] at hk
+          obtain ⟨f, hfm, rfl⟩ := hk
+          have hf := (h f).mp ⟨hfm, hk', hkb⟩
+          apply h'.1.2.2
+          · simpa only [← map_fst_toList_eq_keys] using List.mem_map_of_mem hf.1
+          · exact hf.2.1
+        · refine TransCmp.isLE_trans he.2.2 ?_
+          apply Ordering.isLE_of_eq_lt
+          simpa [OrientedCmp.gt_iff_lt] using hkb
+    simp [this]
+    cases heq : Option.filter (fun e => (cmp e.fst b').isLE) (t'.getEntryGT? a')
+    · simp
+    · rename_i out
+      simp
+      simp [Slice.iter_eq_toIteratorIter, ToIterator.iter_eq, RocSlice.Internal.iterM, Roc.Sliceable.mkSlice,
+        ← hi] at ihy
+      apply ihy (a := out.fst) (a' := out.fst) (b := b) (b' := b') (out := out)
+      · simp [Iter.IsPlausibleStep, IterM.IsPlausibleStep, Iterator.IsPlausibleStep, Iter.toIterM,
+        IterM.toIter]
+        rw [← this, Option.filter_eq_some_iff, and_comm] at heq
+        simpa using heq
+      · intro e
+        have heq' := heq
+        rw [← this, Option.filter_eq_some_iff, getEntryGT?_eq_some_iff] at heq'
+        rw [Option.filter_eq_some_iff, getEntryGT?_eq_some_iff] at heq
+        constructor
+        · intro h'
+          have he := (h e).mp ⟨h'.1, TransCmp.lt_trans heq'.1.2.1 h'.2.1, h'.2.2⟩
+          exact ⟨he.1, h'.2.1, he.2.2⟩
+        · intro h'
+          have he := (h e).mpr ⟨h'.1, TransCmp.lt_trans heq.1.2.1 h'.2.1, h'.2.2⟩
+          exact ⟨he.1, h'.2.1, he.2.2⟩
+      · rfl
 
 public structure RccSliceData (α : Type u) (β : α → Type v)
     (cmp : α → α → Ordering := by exact compare) where
@@ -224,16 +415,22 @@ public theorem val_step_iter_rccSlice_eq_match' {α β} {cmp : α → α → Ord
   · split <;> simp_all [Option.filter_some]
   · simp_all
 
+public theorem filter_toList_eq_match {α β} {cmp : α → α → Ordering} [TransCmp cmp] {t : DTreeMap α β cmp} {a b : α} :
+    t.toList.filter (fun e => (cmp a e.fst).isLE ∧ (cmp e.fst b).isLE) = (match (t.getEntryGE? a).filter (fun e => (cmp e.fst b).isLE) with
+      | some next =>
+        next :: t.toList.filter (fun e => cmp next.fst e.fst = .lt ∧ (cmp e.fst b).isLE)
+      | none =>
+        []) := by
+  sorry
+
 theorem toList_rccSlice_eq_toList_rccSlice {α β} {cmp : α → α → Ordering} [TransCmp cmp] {t t': DTreeMap α β cmp} {a b a' b' : α}
     (h : ∀ c, (c ∈ t.toList ∧ (cmp a c.fst).isLE ∧ (cmp c.fst b).isLE) ↔ (c ∈ t'.toList ∧ (cmp a' c.fst).isLE ∧ (cmp c.fst b').isLE)) :
     t[a...=b].toList = t'[a'...=b'].toList := by
-    -- simp only [Slice.toList_eq_toList_iter, Slice.iter_eq_toIteratorIter, ToIterator.iter_eq,
-    --   RccSlice.Internal.iterM, Rcc.Sliceable.mkSlice, IterM.toIter]
     simp only [Slice.toList_eq_toList_iter]
-    induction hi : Slice.iter (Rcc.Sliceable.mkSlice t a...=b) using Iter.inductSteps
-    rw [← hi]
+    simp only [Slice.iter_eq_toIteratorIter, ToIterator.iter_eq, RccSlice.Internal.iterM, Rcc.Sliceable.mkSlice, IterM.toIter]
     rw [Iter.toList_eq_match_step, Iter.toList_eq_match_step]
-    simp only [val_step_iter_rccSlice_eq_match']
+    rw [val_step_rxcIterator_eq_match', val_step_rxcIterator_eq_match']
+    simp only
     have : (t.getEntryGE? a).filter (fun e => (cmp e.fst b).isLE) =
         (t'.getEntryGE? a').filter (fun e => (cmp e.fst b').isLE) := by
       ext e
@@ -269,54 +466,25 @@ theorem toList_rccSlice_eq_toList_rccSlice {α β} {cmp : α → α → Ordering
           apply Ordering.isLE_of_eq_lt
           simpa [OrientedCmp.gt_iff_lt] using hkb
     simp [this]
-    cases Option.filter (fun e => (cmp e.fst b').isLE) (t'.getEntryGE? a')
+    cases heq : Option.filter (fun e => (cmp e.fst b').isLE) (t'.getEntryGE? a')
     · simp
-    · simp
-
-    match hn : t.getEntryGE? a, hn' : t'.getEntryGE? a' with
-    | none, none => simp
-    | some next, some next' =>
-      have heq : ∀ e, (e ∈ t.toList ∧ (cmp a e.fst).isLE ∧ ∀ k, k ∈ t.keys → (cmp a k).isLE → (cmp e.fst k).isLE) →
-          e = next := by simp [← getEntryGE?_eq_some_iff, hn, Option.some_inj]
-      simp [getEntryGE?_eq_some_iff] at hn hn'
-      have hm : next.fst ∈ t.keys := by simpa only [← map_fst_toList_eq_keys] using List.mem_map_of_mem hn.1
-      have hm' : next'.fst ∈ t'.keys := by simpa only [← map_fst_toList_eq_keys] using List.mem_map_of_mem hn'.1
-      have hle : (cmp next.fst b).isLE → (cmp next'.fst next.fst).isLE := by
-        intro h'
-        have := (h next).mp ⟨hn.1, hn.2.1, h'⟩
-        exact hn'.2.2 next.fst
-          (by simpa only [← map_fst_toList_eq_keys] using List.mem_map_of_mem this.1)
-          this.2.1
-      have hle' : (cmp next'.fst b').isLE → (cmp next.fst next'.fst).isLE := by
-        intro h'
-        have := (h next').mpr ⟨hn'.1, hn'.2.1, h'⟩
-        exact hn.2.2 next'.fst
-          (by simpa only [← map_fst_toList_eq_keys] using List.mem_map_of_mem this.1)
-          this.2.1
-      have : (cmp next.fst b).isLE ↔ (cmp next'.fst b').isLE := by
+    · rename_i out
+      simp
+      have hroc := @toList_rocSlice_eq_toList_rocSlice
+      simp [Slice.toList_eq_toList_iter, Slice.iter_eq_toIteratorIter, ToIterator.iter_eq, RocSlice.Internal.iterM,
+        Roc.Sliceable.mkSlice] at hroc
+      apply hroc
+      · intro e
+        have heq' := heq
+        rw [← this, Option.filter_eq_some_iff, getEntryGE?_eq_some_iff] at heq'
+        rw [Option.filter_eq_some_iff, getEntryGE?_eq_some_iff] at heq
         constructor
         · intro h'
-          have := (h next).mp ⟨hn.1, hn.2.1, h'⟩
-          exact TransCmp.isLE_trans (hle h') this.2.2
+          have he := (h e).mp ⟨h'.1, TransCmp.isLE_trans heq'.1.2.1 (Ordering.isLE_of_eq_lt h'.2.1), h'.2.2⟩
+          exact ⟨he.1, h'.2.1, he.2.2⟩
         · intro h'
-          have := (h next').mpr ⟨hn'.1, hn'.2.1, h'⟩
-          exact TransCmp.isLE_trans (hle' h') this.2.2
-      by_cases h' : (cmp next.fst b).isLE
-      · have : next' = next := by
-          apply heq
-          have h'' := this.mp h'
-          have := (h next').mpr ⟨hn'.1, hn'.2.1, h''⟩
-          refine ⟨this.1, this.2.1, ?_⟩
-          intro k hk hk'
-          exact TransCmp.isLE_trans (hle h') (hn.2.2 k hk hk')
-        cases this
-        simp [h', this.mp h']
-      · have : ¬ (cmp next'.fst b').isLE := by simpa [this] using h'
-        simp [h', this]
-    | none, some x =>
-      sorry
-    | some x, none =>
-      sorry
+          have he := (h e).mpr ⟨h'.1, TransCmp.isLE_trans heq.1.2.1 (Ordering.isLE_of_eq_lt h'.2.1), h'.2.2⟩
+          exact ⟨he.1, h'.2.1, he.2.2⟩
 
 theorem rccSlice_toList_eq_filter_toList {α β} {cmp : α → α → Ordering} [TransCmp cmp] {t : DTreeMap α β cmp} {a b : α} :
     t[a...=b].toList = t.toList.filter (fun e => (cmp a e.fst).isLE ∧ (cmp e.fst b).isLE)
